Add Equals methods

IntegerSet/dafny/TreeSet.dfy
@@ -12,7 +12,36 @@ module TreeSet {
     }
 
     datatype Tree = Leaf | Node(left : Tree, value : int, right : Tree)
-        
+
+    //region ordered
+    function lesser(t : Tree, i : int) : bool {
+        t.Leaf? || (i < t.value && lesser(t.left, i) && lesser(t.right, i))
+    }
+    function greater(t : Tree, i : int) : bool {
+        t.Leaf? || (i > t.value && greater(t.left, i) && greater(t.right, i))
+    }
+    function ordered(t : Tree) : bool {
+        if(t.Node?)
+        then greater(t.left, t.value) && lesser(t.right, t.value)
+        else true
+    }
+    //endregion
+
+    //region unique
+    function count(t : Tree, i : int) : (count : int) 
+    ensures count >= 0
+    {
+        if(t.Node?)
+        then (if(t.value == i) then 1 else 0) + count(t.left, i) + count(t.right, i)
+        else 0
+    }
+    function unique(t : Tree) : bool {
+        if(t.Node?)
+        then count(t, t.value) == 1 && unique(t.left) && unique(t.right)
+        else true
+    }
+    //endregion unique
+
     function copy(t : Tree) : (o : Tree) 
     ensures unique(t) && ordered(t) <==> unique(o) && ordered(o)
     ensures size(t) == size(o)
@@ -20,6 +49,25 @@ module TreeSet {
         if(t.Node?)
         then Node(copy(t.left), t.value, copy(t.right))
         else Leaf
+    }
+
+    function size(t : Tree) : (s : int)
+    ensures s >= 0
+    {
+        if(t.Node?)
+        then size(t.left) + size(t.right) + 1
+        else 0
+    }
+
+    //region CRUD
+    function containsElement(t : Tree, i : int) : bool  
+    requires unique(t) && ordered(t)
+    {
+        t.Node? && (i == t.value || (
+            if(i < t.value)
+            then containsElement(t.left, i)
+            else containsElement(t.right, i)
+        ))
     }
 
     function addElement(t : Tree, i : int) : (o : Tree) 
@@ -40,6 +88,60 @@ module TreeSet {
         )
         else Node(Leaf, i, Leaf)
     }
+
+    function removeElement(t : Tree, i : int) : (o : Tree) 
+    requires unique(t) && ordered(t)
+    ensures  !containsElement(o, i)
+    ensures  unique(o) && ordered(o)
+    ensures  (containsElement(t, i) && size(t) + 1 == size(o)) || size(t) == size(o)
+    {
+        if(t.Node?)
+        then (
+            if(i == t.value)
+            then union(t.left, t.right)
+            else (
+                if(i < t.value)
+                then Node(removeElement(t.left, i), t.value, copy(t.right))
+                else Node(copy(t.left), t.value, removeElement(t.right, i))
+            )
+        )
+        else Node(Leaf, i, Leaf)
+    }
+    //endregion
+
+    //region Set Functions
+    function strictEquals(l : Tree, r : Tree) : (b : bool)
+    ensures b ==> (size(l) == size(r))
+    ensures b <==> equals(l, r)
+    {
+        if(l.Node? && r.Node?)
+        then(
+            if(l.value == r.value)
+            then (strictEquals(l.left, r.left) && strictEquals(l.right, r.right))
+            else false
+        )
+        else false
+    }
+
+    //region equals
+    function containsAll(l : Tree, r : Tree) : (b : bool)
+    requires unique(l) && ordered(l)
+    requires unique(r) && ordered(r)
+    ensures b <==> (forall i :: containsElement(r, i) ==> containsElement(l, i))
+    ensures b ==> (size(l) >= size(r))
+    {
+        r.Leaf? || (containsElement(l, r.value) && containsAll(l, r.left) && containsElement(r, r.right))
+    }
+
+    function equals(l : Tree, r : Tree) : (b : bool)
+    requires unique(l) && ordered(l)
+    requires unique(r) && ordered(r)
+    ensures b <==> (forall i :: containsElement(l, i) <==> containsElement(r, i))
+    ensures b ==> (size(l) == size(r))
+    {
+        containsAll(l, r) && size(l) == size(r)
+    }
+    //endregion
 
     function intersect(l : Tree, r : Tree) : (t : Tree)  
     requires unique(l) && ordered(l)  
@@ -84,67 +186,5 @@ module TreeSet {
         )
         else Leaf
     }
-
-    function removeElement(t : Tree, i : int) : (o : Tree) 
-    requires unique(t) && ordered(t)
-    ensures  !containsElement(o, i)
-    ensures  unique(o) && ordered(o)
-    ensures  (containsElement(t, i) && size(t) + 1 == size(o)) || size(t) == size(o)
-    {
-        if(t.Node?)
-        then (
-            if(i == t.value)
-            then union(t.left, t.right)
-            else (
-                if(i < t.value)
-                then Node(removeElement(t.left, i), t.value, copy(t.right))
-                else Node(copy(t.left), t.value, removeElement(t.right, i))
-            )
-        )
-        else Node(Leaf, i, Leaf)
-    }
-
-    function containsElement(t : Tree, i : int) : bool  
-    requires unique(t) && ordered(t)
-    {
-        t.Node? && (i == t.value || (
-            if(i < t.value)
-            then containsElement(t.left, i)
-            else containsElement(t.right, i)
-        ))
-    }
-    
-    function lesser(t : Tree, i : int) : bool {
-        t.Leaf? || (i < t.value && lesser(t.left, i) && lesser(t.right, i))
-    }
-    function greater(t : Tree, i : int) : bool {
-        t.Leaf? || (i > t.value && greater(t.left, i) && greater(t.right, i))
-    }
-    function ordered(t : Tree) : bool {
-        if(t.Node?)
-        then greater(t.left, t.value) && lesser(t.right, t.value)
-        else true
-    }
-
-    function count(t : Tree, i : int) : (count : int) 
-    ensures count >= 0
-    {
-        if(t.Node?)
-        then (if(t.value == i) then 1 else 0) + count(t.left, i) + count(t.right, i)
-        else 0
-    }
-
-    function unique(t : Tree) : bool {
-        if(t.Node?)
-        then count(t, t.value) == 1 && unique(t.left) && unique(t.right)
-        else true
-    }
-
-    function size(t : Tree) : (s : int)
-    ensures s >= 0
-    {
-        if(t.Node?)
-        then size(t.left) + size(t.right) + 1
-        else 0
-    }
+    //endregion
 }
